cfrontend/Ctyping.v
@@ -1693,14 +1693,14 @@ Lemma wt_deref_loc:
 Proof.
   induction 1.
 - (* by value, non volatile *)
-  simpl in H1. exploit Mem.load_result; eauto. intros EQ; rewrite EQ.
+  exploit Mem.load_result; eauto with mem. intros EQ; rewrite EQ.
   apply wt_decode_val; auto.
 - (* by value, volatile *)
   inv H1.
   + (* truly volatile *)
     eapply wt_load_result; eauto.
   + (* not really volatile *)
-    exploit Mem.load_result; eauto. intros EQ; rewrite EQ.
+    exploit Mem.load_result; eauto with mem. intros EQ; rewrite EQ.
     apply wt_decode_val; auto.
 - (* by reference *)
   destruct ty; simpl in H; try discriminate; auto with ty.
